\begin{zsection}
\SECTION simple2 \parents zpattern\_toolkit
\end{zsection}

\begin{zedjoker}{DeclList} D, D1, D2, D3\end{zedjoker} \\
\begin{zedjoker}{Pred} P, P1, P2\end{zedjoker} \\
\begin{zedjoker}{Expr} E, E2\end{zedjoker} \\
\begin{zedjoker}{Name} v\end{zedjoker} \\

We define an infix operator for unfolding schemas.


\newcommand{\unfoldsTo}{\mathrel{\leadsto}}

\begin{verbatim}
%%Zinword \unfoldsTo unfoldsTo
\end{verbatim}

\begin{zed}
  \relation ( \_ \unfoldsTo \_ )
\end{zed}

\begin{gendef}[SCHEMA]
  \_ \unfoldsTo \_ : SCHEMA \rel SCHEMA
\where
  \forall s1,s2:SCHEMA @ s1 \unfoldsTo s2 \iff s1=s2
\end{gendef}


\begin{schema}{Foo}
  x:\nat
\where
  true
\end{schema}

\begin{zed}
  \relation ( \_~foo~\_ )
\end{zed}

\begin{gendef}[SCHEMA]
  \_ ~foo~ \_ : SCHEMA \rel SCHEMA
\where
  \forall s1,s2:SCHEMA @ s1 ~foo~ s2 \iff s1=s2
\end{gendef}

\begin{zedrule}{test}
  [ v:E ; D | P1 ] foo~ E2
\end{zedrule}

\begin{zed}
  \vdash?~ [ x:\nat | true ] ~foo~ [ x:\nat | true ]
\end{zed}

\begin{zed}
  \vdash?~ [ x:\nat; y:\nat | true ] ~foo~ [ x:\nat; y:\nat | true ]
\end{zed}

\begin{zed}
  \vdash?~ [ x:\nat; y:\nat ; Foo | true ] ~foo~
           [ x:\nat; y:\nat ; Foo | true ]
\end{zed}


\begin{zedrule}{argh}
  [ v ; D | P1 ] ~foo~ E2
\end{zedrule}

\begin{zed}
  \vdash?~ [Foo | true] ~foo~ [Foo | true]
\end{zed}

\begin{zed}
  \vdash?~ [Foo ; x,y:\nat | true] ~foo~ [Foo ; x,y:\nat | true]
\end{zed}

\begin{zedrule}{test2}
  [ v:E ; D | P1 ] = [ v:E ; D | P1 ]
\end{zedrule}

\begin{zed}
  \vdash?~ [ x:\nat | true ] = [ x:\nat | true ]
\end{zed}

\begin{zed}
  \vdash?~ [ x:\nat; y:\nat | true ] = [ x:\nat; y:\nat | true ]
\end{zed}

\begin{zed}
  \vdash?~ [ x:\nat; y:\nat ; z:\nat | true ] =
           [ x:\nat; y:\nat ; z:\nat | true ]
\end{zed}



\begin{zedrule}{normaliseEmpty}
   [~ | true] \unfoldsTo [~ | true]
\end{zedrule}

\begin{zedrule}{normaliseVarDecl}
   [D1 | true] \unfoldsTo [D2 | P2]
\derives
   [v:E; D1 | true] \unfoldsTo [v:E; D2 | P2]
\end{zedrule}

\begin{zedrule}{startNormalise}
   [D1 | true] \unfoldsTo [D2 | P2]
\derives
   [D1 | P] = [D2 | P2 \land P]
\end{zedrule}

\begin{zed}
  \vdash?~ [~ | true] = [~ | true \land true]
\end{zed}

\begin{zed}
  \vdash?~ [x:\nat | true] = [x:\nat | true \land true]
\end{zed}

\begin{zed}
  \vdash?~ [x:\nat ; y:\nat | true] = [x:\nat ; y:\nat | true \land true]
\end{zed}

\begin{zed}
  \vdash?~ [x:\nat ; y:\nat ; z:\nat | true] =
           [x:\nat ; y:\nat ; z:\nat | true \land true]
\end{zed}



\begin{zedrule}{normaliseIncludeDecl}
   \proviso ?~ v == [D1 | P1] \\
\derives
   [v; D | true] \unfoldsTo [D1 | P1 \land P2]
\end{zedrule}

\begin{zed}
  \vdash?~ [ Foo | true ] \unfoldsTo [ x:\nat | true \land true ]
\end{zed}